newio/Hist.fst
@@ -15,66 +15,66 @@ The history is in reverse chronological order.
 At the end of an io computation, the local trace is
 reversed and appended to the history. **)
 
-let hist_post (#event:Type) a = lt:list event -> r:a -> Type0
-let hist_pre (#event:Type) = h:list event -> Type0
+let hist_post (#event_type:Type) a = lt:list event_type -> r:a -> Type0
+let hist_pre (#event_type:Type) = h:list event_type -> Type0
 
-private let hist0 (#event:Type) a = hist_post #event a -> hist_pre #event
+private let hist0 (#event_type:Type) a = hist_post #event_type a -> hist_pre #event_type
 
 unfold
-let hist_post_ord (#event:Type) (p1 p2:hist_post #event 'a) = forall lt r. p1 lt r ==> p2 lt r
+let hist_post_ord (#event_type:Type) (p1 p2:hist_post #event_type 'a) = forall lt r. p1 lt r ==> p2 lt r
 
-let hist_wp_monotonic (#event:Type) (wp:hist0 #event 'a) =
+let hist_wp_monotonic (#event_type:Type) (wp:hist0 #event_type 'a) =
   forall p1 p2. (p1 `hist_post_ord` p2) ==> (forall h. wp p1 h ==> wp p2 h)
 
-let hist #event a = wp:(hist0 #event a){hist_wp_monotonic wp}
+let hist #event_type a = wp:(hist0 #event_type a){hist_wp_monotonic wp}
 
-val hist_subcomp0 : #event:Type -> #a:Type -> #p1:(a -> Type0) -> #p2:(a -> Type0) -> #_:unit{forall x. p1 x ==> p2 x} -> wp:hist #event (x:a{p1 x}) -> 
-  (hist #event (x:a{p2 x}))
+val hist_subcomp0 : #event_type:Type -> #a:Type -> #p1:(a -> Type0) -> #p2:(a -> Type0) -> #_:unit{forall x. p1 x ==> p2 x} -> wp:hist #event_type (x:a{p1 x}) -> 
+  (hist #event_type (x:a{p2 x}))
 let hist_subcomp0 #_ #a #p1 #p2 #_ wp : (hist (x:a{p2 x})) =
   let wp' : hist0 (x:a{p2 x}) = wp in
   assert (forall (post1:hist_post (x:a{p2 x})) (post2:hist_post (x:a{p2 x})). (hist_post_ord post1 post2 ==> (forall h. wp' post1 h ==> wp' post2 h)));
   assert (hist_wp_monotonic #(x:a{p2 x}) wp');
   wp'
 
-val hist_subcomp : #event:Type -> #a:Type -> #p1:(a -> Type0) -> #p2:(a -> Type0) -> wp:hist #event (x:a{p1 x}) -> 
-  Pure (hist #event (x:a{p2 x})) (requires (forall x. p1 x ==> p2 x)) (ensures (fun _ -> True))
-let hist_subcomp #event #a #p1 #p2 wp = hist_subcomp0 #event #a #p1 #p2 #() wp
+val hist_subcomp : #event_type:Type -> #a:Type -> #p1:(a -> Type0) -> #p2:(a -> Type0) -> wp:hist #event_type (x:a{p1 x}) -> 
+  Pure (hist #event_type (x:a{p2 x})) (requires (forall x. p1 x ==> p2 x)) (ensures (fun _ -> True))
+let hist_subcomp #event_type #a #p1 #p2 wp = hist_subcomp0 #event_type #a #p1 #p2 #() wp
 
 
-let hist_return (#event:Type) (x:'a) : hist #event 'a =
+let hist_return (#event_type:Type) (x:'a) : hist #event_type 'a =
   fun p _ -> p [] x
 
 unfold
-let hist_post_shift (#event:Type) (p:hist_post #event 'a) (lt:list event) : hist_post #event 'a =
+let hist_post_shift (#event_type:Type) (p:hist_post #event_type 'a) (lt:list event_type) : hist_post #event_type 'a =
   fun lt' r -> p (lt @ lt') r
 
 unfold
 let hist_post_bind
-  (#event:Type)
-  (h:list event)
-  (kw : 'a -> hist #event 'b)
-  (p:hist_post #event 'b) :
-  Tot (hist_post #event 'a) =
+  (#event_type:Type)
+  (h:list event_type)
+  (kw : 'a -> hist #event_type 'b)
+  (p:hist_post #event_type 'b) :
+  Tot (hist_post #event_type 'a) =
   fun lt r ->
     kw r (hist_post_shift p lt) (List.rev lt @ h)
 
 unfold
-let hist_bind (#event:Type) (a b:Type) (w : hist #event a) (kw : a -> hist #event b) : hist #event b =
-  fun p h -> w (hist_post_bind #a #b #event h kw p) h
+let hist_bind (#event_type:Type) (a b:Type) (w : hist #event_type a) (kw : a -> hist #event_type b) : hist #event_type b =
+  fun p h -> w (hist_post_bind #a #b #event_type h kw p) h
 
 unfold
-let wp_lift_pure_hist (#event:Type) (w : pure_wp 'a) : hist #event 'a =
+let wp_lift_pure_hist (#event_type:Type) (w : pure_wp 'a) : hist #event_type 'a =
   FStar.Monotonic.Pure.elim_pure_wp_monotonicity_forall ();
   fun p _ -> w (p [])
 
-let lemma_wp_lift_pure_hist_implies_as_requires #a #event w :
-  Lemma (forall (p:hist_post #event a) h. wp_lift_pure_hist w p h ==> as_requires w) =
-    assert (forall (p:hist_post #event a) x. p [] x ==> True) ;
+let lemma_wp_lift_pure_hist_implies_as_requires #a #event_type w :
+  Lemma (forall (p:hist_post #event_type a) h. wp_lift_pure_hist w p h ==> as_requires w) =
+    assert (forall (p:hist_post #event_type a) x. p [] x ==> True) ;
     FStar.Monotonic.Pure.elim_pure_wp_monotonicity w ;
-    assert (forall (p:hist_post #event a). w (fun x -> p [] x) ==> w (fun _ -> True))
+    assert (forall (p:hist_post #event_type a). w (fun x -> p [] x) ==> w (fun _ -> True))
 
 unfold
-val hist_ord (#event:Type) (#a : Type) : hist #event a -> hist #event a -> Type0
+val hist_ord (#event_type:Type) (#a : Type) : hist #event_type a -> hist #event_type a -> Type0
 let hist_ord wp1 wp2 = forall h p. wp1 p h ==> wp2 p h
 
 unfold
